\ifnum \Version=1    
\question[2] You do not need to show your work for this question. Complete the table below by calculating the inverse Laplace Transform of the following functions. 
\vspace{-0.2cm}
\setlength{\extrarowheight}{0.60cm}
\begin{center}
\hspace{-.9cm}\begin{tabular}{ p{0.20cm} p{4cm} p{7cm}  }
    & $F(s) = \mathcal{L} [f(t)]$& $f(t)$   \\[2pt] \hline 
    % a) & $\displaystyle F(s) = \frac{1}{s^2+4}$ & $f(t) = $ \\[4pt]  
    a) & $\displaystyle F(s) = \frac{e^{-3s}}{s^2+4}$ & $f(t) = $ \ifnum \Solutions=1 {\color{DarkBlue}  $\frac12 u_3\sin(2(t-3))$ }\fi \\[4pt] 
    b) & $\displaystyle F(s) = \frac{2}{s}+\frac{3}{s+4}$  & $f(t) = $ \ifnum \Solutions=1 {\color{DarkBlue} $2+3e^{-4t}$}\fi \\[12pt] 
    \hline
\end{tabular}
\end{center}
\setlength{\extrarowheight}{0.0cm}
\fi 


\ifnum \Version=2
\question[2] You do not need to show your work for this question. Complete the table below by calculating the inverse Laplace Transform of the following functions. 
\vspace{-0.2cm}
\setlength{\extrarowheight}{0.60cm}
\begin{center}
\hspace{-.9cm}\begin{tabular}{ p{0.20cm} p{4cm} p{7cm}  }
    & $F(s) = \mathcal{L} [f(t)]$& $f(t)$   \\[2pt] \hline 
    a) & $\displaystyle F(s) = \frac{6e^{-4s}}{s-3}$ & $f(t) = $ \ifnum \Solutions=1 {\color{DarkBlue}  $6u_4e^{3(t-4)}$ }\fi \\[4pt] 
    b) & $\displaystyle F(s) = \frac{3}{(s+1)^2+4}$ & $f(t) = $ \ifnum \Solutions=1 {\color{DarkBlue} $\frac32e^{-t}\sin(2t)$}\fi \\[8pt]      
    \hline
\end{tabular}
\end{center}
\setlength{\extrarowheight}{0.0cm}
\fi 



\ifnum \Version=3
\question[2] You do not need to show your work for this question. Complete the table below by calculating the inverse Laplace Transform of the following functions. 
\vspace{-0.2cm}
\setlength{\extrarowheight}{0.60cm}
\begin{center}
\hspace{-.9cm}\begin{tabular}{ p{0.20cm} p{4cm} p{7cm}  }
    & $F(s) = \mathcal{L} [f(t)]$& $f(t)$   \\[2pt] \hline 
    a) & $\displaystyle F(s) = \frac{s}{(s+1)^2+4}$ & $f(t) = $ \ifnum \Solutions=1 {\color{DarkBlue} $e^{-t}\cos(2t) - \frac12 e^{-t}\sin(2t) $}\fi \\[8pt]     
    b) & $\displaystyle F(s) = \frac{6e^{-4s}}{s-3}$ & $f(t) = $ \ifnum \Solutions=1 {\color{DarkBlue}  $6u_4e^{3(t-4)}$ }\fi \\[4pt]      
    \hline
\end{tabular}
\end{center}
\setlength{\extrarowheight}{0.0cm}
\ifnum \Solutions=1 {\color{DarkBlue}
Note that: $\displaystyle F(s) = \frac{s}{(s+1)^2+4} = \frac{s+1-1}{(s+1)^2+2^2} = \frac{s+1}{(s+1)^2+2^2  } - \frac12 \frac{2}{(s+1)^2+2^2}$
} 
\else 
\fi
\fi 

\ifnum \Version=4
\question[2] You do not need to show your work for this question. Complete the table below by calculating the inverse Laplace Transform of the following functions. 
\vspace{-0.2cm}
\setlength{\extrarowheight}{0.60cm}
\begin{center}
\hspace{-.9cm}\begin{tabular}{ p{0.20cm} p{4cm} p{7cm}  }
    & $F(s) = \mathcal{L} [f(t)]$& $f(t)$   \\[2pt] \hline 
    a) & $\displaystyle F(s) = \frac{4s}{(s+3)^2+16}$ & $f(t) = $ \ifnum \Solutions=1 {\color{DarkBlue}$ 4e^{-3t}\cos(4t) - 3e^{-3t}\sin(4t)$}\fi \\[4pt]     
    b) & $\displaystyle F(s) = \frac{6e^{-4s}}{s-3}$ & $f(t) = $ \ifnum \Solutions=1 {\color{DarkBlue}  $6u_4 e^{3(t-4)}$ }\fi \\[8pt]      
    \hline
\end{tabular}
\end{center}
\setlength{\extrarowheight}{0.0cm}
\ifnum \Solutions=1 {\color{DarkBlue}
Note that: $\displaystyle F(s) = \frac{4s}{(s+3)^2+16} = \frac{4(s+3-3)}{(s+3)^2+4^2} = \frac{4(s+3)}{(s+3)^2+4^2  } - \frac{3\cdot4}{(s+3)^2+4^2}$
} 
\else 
\fi
\fi 

\ifnum \Version=5
\question[2] You do not need to show your work for this question. Complete the table below by calculating the inverse Laplace Transform of the following functions. 
\vspace{-0.2cm}
\setlength{\extrarowheight}{0.60cm}
\begin{center}
\hspace{-.9cm}\begin{tabular}{ p{0.20cm} p{4cm} p{7cm}  }
    & $F(s) = \mathcal{L} [f(t)]$& $f(t)$   \\[2pt] \hline 
    a) & $\displaystyle F(s) = \frac{2e^{-6s}}{s+3}$ & $f(t) = $ \ifnum \Solutions=1 {\color{DarkBlue}  $2u_6e^{-3(t-6)}$ }\fi \\[4pt]      
    b) & $\displaystyle F(s) = \frac{4s}{(s+3)^2+16}$ & $f(t) = $ \ifnum \Solutions=1 {\color{DarkBlue} $ 4e^{-3t}\cos(4t) - 3e^{-3t}\sin(4t)$}\fi \\[8pt]     
    \hline
\end{tabular}
\end{center}
\setlength{\extrarowheight}{0.0cm}
\ifnum \Solutions=1 {\color{DarkBlue}
Note that: $\displaystyle F(s) = \frac{4s}{(s+3)^2+16} = \frac{4(s+3-3)}{(s+3)^2+4^2} = \frac{4(s+3)}{(s+3)^2+4^2  } - \frac{3\cdot4}{(s+3)^2+4^2}$
} 
\else 
\fi
\fi 


\ifnum \Version=6
\question[3] You do not need to show your work for this question. Complete the table below by calculating the inverse Laplace Transform of the following functions. 
\vspace{-0.6cm}
\setlength{\extrarowheight}{0.60cm}
\begin{center}
\hspace{-.9cm}\begin{tabular}{ p{0.20cm} p{4cm} p{7cm}  }
    & $F(s) = \mathcal{L} [f(t)]$& $f(t)$   \\[2pt] \hline 
    a) & $\displaystyle F(s) = \frac{3e^{-6s}}{s+12}$ & $f(t) = $ \ifnum \Solutions=1 {\color{DarkBlue}  $3u_{6}e^{-12(t-6)}$ }\fi \\[4pt]      
    b) & $\displaystyle F(s) = \frac{4s}{(s+2)^2+9}$ & $f(t) = $ \ifnum \Solutions=1 {\color{DarkBlue} $ 4e^{-2t}\cos(3t) - \frac83e^{-2t}\sin(3t)$}\fi \\[4pt]     
    c) & $\displaystyle F(s) = \frac{4s+2}{s^2+16}$ & $f(t) = $ \ifnum \Solutions=1 {\color{DarkBlue} $ 4\cos(4t) + \frac12 \sin(4t)$}\fi \\[8pt]         
    \hline
\end{tabular}
\end{center}
\setlength{\extrarowheight}{0.0cm}
\ifnum \Solutions=1 {\color{DarkBlue}
Note that: 
\begin{align}
    \frac{4s}{(s+2)^2+9} &= \frac{4(s+2-2)}{(s+2)^2+3^2} = \frac{4(s+2)}{(s+2)^2+3^2  } - \frac83\frac{3}{(s+2)^2+3^2}\\
\end{align}
} 
\else 
\fi
\fi 


\ifnum \Version=7
\question[3] You do not need to show your work for this question. Complete the table below by calculating the inverse Laplace Transform of the following functions. 
\vspace{-0.2cm}
\setlength{\extrarowheight}{0.60cm}
\begin{center}
\hspace{-.9cm}\begin{tabular}{ p{0.20cm} p{4cm} p{7cm}  }
    & $F(s) = \mathcal{L} [f(t)]$& $f(t)$   \\[2pt] \hline 
    a) & $\displaystyle F(s) = \frac{4s}{(s+3)^2+16}$ & $f(t) = $ \ifnum \Solutions=1 {\color{DarkBlue}$ 4e^{-3t}\cos(4t) - 3e^{-3t}\sin(4t)$}\fi \\[4pt]     
    b) & $\displaystyle F(s) = \frac{6e^{-4s}}{s-3}$ & $f(t) = $ \ifnum \Solutions=1 {\color{DarkBlue}  $6u_4 e^{3(t-4)}$ }\fi \\[4pt]      
    c) & $\displaystyle F(s) = \frac{4s+2}{s^2+9}$ & $f(t) = $ \ifnum \Solutions=1 {\color{DarkBlue} $ 4e^{-3t}\cos(4t) - 3e^{-3t}\sin(4t)$}\fi \\[8pt]             
    \hline
\end{tabular}
\end{center}
\setlength{\extrarowheight}{0.0cm}
\ifnum \Solutions=1 {\color{DarkBlue}
Note that: $\displaystyle F(s) = \frac{4s}{(s+3)^2+16} = \frac{4(s+3-3)}{(s+3)^2+4^2} = \frac{4(s+3)}{(s+3)^2+4^2  } - \frac{3\cdot4}{(s+3)^2+4^2}$
} 
\else 
\fi
\fi 