%\vfill\rightline{(See the next page for the answers)}

\newpage

\item
	 
	\begin{enumerate}
	\item
The general solutions: 
$\bmatrix{x_1(t)\cr x_2(t)}
=
C_1 e^{3t} \bmatrix{2\cr 1}  
+C_2 e^{3t} \left(  \bmatrix{-1\cr 0} + t\bmatrix{2\cr 1} \right)$.
\\
% where $C_1,C_2$ are free parameters.\\
The solution satisfying $x_1(0)=-1,x_2(0)=2$ is
$\bmatrix{x_1(t)\cr x_2(t)}
=\bmatrix{-e^{3t}+10te^{3t} \cr 2e^{3t}+5te^{3t}}$.\\
The equilibrium $(x_1,x_2)=(0,0)$ 
is a repulsive degenerate node and is unstable.
\medskip

\begin{minipage}{0.68\textwidth}
{\color{red}\small\em Notes:}
	{\small \color{blue}
The phase portrait
should show the following elements:
\begin{description}
\item{$\bullet$}
the correct eigenspace in the direction of 
$\bmatrix{2\cr 1}$;
\item{$\bullet$}
trajectories that are not on
the eigenspace are U-turn shaped curves,
emanating from the origin;
\item{$\bullet$} 
at the equilibrium, all the curved trajectories are tangent 
to the eigenspace;
\item{$\bullet$}
and needless to say, the correct arrows
on all trajectories.
\end{description}}
\end{minipage}
\hfill
\begin{minipage}{0.3\textwidth}
\includegraphics*[width=\textwidth]{testpr-repulsive-degenerate-node.eps}
\end{minipage}

	\item
The general solutions: 
$\bmatrix{x_1(t)\cr x_2(t)}
=C_1 e^{-3t} \bmatrix{-1/2\cr 1}  
+C_2 e^{-3t} \left(  \bmatrix{1/4\cr 0} + t\bmatrix{-1/2\cr 1} \right)$.\\
The solution satisfying $x_1(0)=-1,x_2(0)=2$ is
$\bmatrix{x_1(t)\cr x_2(t)}
=\bmatrix{-e^{-3t}  \cr 2e^{-3t} }$.\\
The equilibrium $(x_1,x_2)=(0,0)$ 
is an attractive degenerate node
and is asymptotically stable.
\medskip

\begin{minipage}{0.68\textwidth}
{\color{red}\small\em Notes:}
	{\small \color{blue}
The phase portrait
should show the following elements:
\begin{description}
\item{$\bullet$}
the correct eigenspace in the direction of 
$\bmatrix{-1/2\cr 1}$;
\item{$\bullet$}
trajectories that are not on 
the eigenspace are U-turn shaped curves,
converging to the origin;
\item{$\bullet$} 
at the equilibrium, all the curved trajectories are tangent 
to the eigenspace;
\item{$\bullet$}
and needless to say, the correct arrows
on all trajectories.
\end{description}}
\end{minipage}
\hfill
\begin{minipage}{0.3\textwidth}
\includegraphics*[width=\textwidth]{testpr-attractive-degenerate-node.eps}
\end{minipage}

\medskip

% ${ }$
% \\[-1.em]
\begin{minipage}{0.68\textwidth}
	\item
The general solutions: 
$\bmatrix{x_1(t)\cr x_2(t)}
=C_1 e^{-2t} \bmatrix{1\cr 0}  
+C_2 e^{-2t} \bmatrix{0\cr 1} $.\\
The solution satisfying $x_1(0)=-1,x_2(0)=2$ is
$\bmatrix{x_1(t)\cr x_2(t)}
=\bmatrix{-e^{-2t}  \cr 2e^{-2t}}$.\\
The equilibrium $(x_1,x_2)=(0,0)$ 
is an attractive proper node
and is asymptotically stable.
\end{minipage}
\hfill
\begin{minipage}{0.3\textwidth}
\includegraphics*[width=\textwidth]{testpr-attractive-proper-node.eps}
\end{minipage}

	\end{enumerate} 

%% \newpage
%\item
 
${ }$
\\[-1.em]
\begin{minipage}{0.68\textwidth}
\item
(a) Only one equilbrium: $(1,-2)$
\\
The general solutions:\\
$\bmatrix{x_1(t)\cr x_2(t)}
=\bmatrix{1\cr -2} 
+C_1 e^{-2t}\left( \cos(5t)\bmatrix{-1\cr 1} -\sin(5t)\bmatrix{-1\cr 0} \right)\\
+C_2 e^{-2t}\left( \sin(5t)\bmatrix{-1\cr 1} +\cos(5t)\bmatrix{-1\cr 0} \right)$,\\
where $C_1,C_2$ are free parameters.\\
The sol satisfying $x_1(0)=2$, $x_2(0)=1$ is\\
$\bmatrix{x_1(t)\cr x_2(t)}
=\bmatrix{1  +e^{-2t} \cos(5t) +7e^{-2t} \sin(5t)\cr 
          -2+3e^{-2t} \cos(5t) -4e^{-2t} \sin(5t)}$.\\
The equilibrium $(x_1,x_2)=(1,-2)$ 
is an attractive focus and is asymptotically stable.
\end{minipage}
\begin{minipage}{0.3\textwidth}
\includegraphics*[width=\textwidth]{testpr-shifted-attractive-focus.eps}
\end{minipage}

 
\begin{minipage}{0.68\textwidth}
(b) Only one equilbrium: $(1,1)$
\\
The general solutions:
$\bmatrix{x_1(t)\cr x_2(t)}
=\bmatrix{1\cr 1} + 
C_1 e^{3t} \bmatrix{2\cr 1} +C_2 e^{-3t} \bmatrix{-1\cr 1}$,
where $C_1,C_2$ are free parameters.\\
The solution satisfying $x_1(0)=2,x_2(0)=1$ is\\
$\bmatrix{x_1(t)\cr x_2(t)}
=\bmatrix{1\cr 1}
 +\frac{1}{3}e^{3t}\bmatrix{2\cr 1} -\frac{1}{3} e^{-3t} \bmatrix{-1\cr 1}$.\\
The equilibrium $(x_1,x_2)=(1,1)$ is a saddle and is unstable.
\end{minipage}
\begin{minipage}{0.3\textwidth}
\rightline{\includegraphics*[width=\textwidth]{testpr-shifted-saddle.eps}}
\end{minipage}
	 


%%% A tank system with two distinct negative eigenvalues

\item
	\begin{enumerate}
	\item
$x_1'=-\frac{1}{20}x_1,\ 
x_2'=\frac{1}{20}x_1-\frac{1}{10}x_2,\ 
x_1(0)=10\mbox{\rm ~lb},\ x_2(0)=0$
	\item
$x_1(t)=10e^{-t/20}\mbox{\rm ~lb},
x_2(t)=10e^{-t/20} -10e^{-t/10} \mbox{\rm ~lb}$
	\item
$\displaystyle \max_{t\ge 0} x_2(t)=x_2(20\ln 2)=2.5 \mbox{\rm ~lb}$
	\end{enumerate}


%%% A tank system with repeated eigenvalues
\def\TANKSREPEATEDANS{
\item
(a) $x_1(t)=10e^{-t/20}\mbox{\rm ~lb},
x_2(t)={1\over 2}te^{-t/20}\mbox{\rm ~lb}$
\\ 
(b) $\displaystyle \max_{t\ge 0} x_2(t)=x_2(20)=10/e \mbox{\rm ~lb}$
(that's $ \approx 3.68 \mbox{\rm ~lb})$
}
 



\item
	\begin{enumerate}
	\item
Substitute $y_1$ and $y_2$ in $(*)$ and simplify.
Details skipped here.
	\item
$y(t)=C_1(1+t^2)+C_2 e^{-t}$ where $C_1$ and $C_2$ are free parameters.
	\item
$y(t)=3(1+t^2) -2 e^{-t}$
	\item
Set $x_1=y,x_2=y'$. The equivalent system is:
$$
\bmatrix{x_1'\cr x_2'}=
\bmatrix{ 
0 & 1 \cr
\frac{2}{1+t} & \frac{1-t}{1+t}
}
\bmatrix{x_1\cr x_2}.
$$
The general solutions of this system are
$\bmatrix{x_1(t)\cr x_2(t)} =
\bmatrix{ C_1(1+t^2)+C_2 e^{-t} \cr 2C_1 t -C_2 e^{-t}}$.
Or, equivalently,
$\bmatrix{x_1(t)\cr x_2(t)} =
C_1 \bmatrix{1+t^2 \cr 2t} +C_2\bmatrix{e^{-t}\cr -e^{-t}}$.
	\item
Substitute $y_0$ in $(**)$ and simplify.
Details skipped here.	
	\item
$y(t)=e^{2t}+ C_1(1+t^2)+C_2 e^{-t}$ where $C_1$ and $C_2$ are free parameters.
	\item
$y(t)=e^{2t}+ 9(1+t^2) -3 e^{-t}$
	\item
Set $x_1=y,x_2=y'$. The equivalent system is:
$$
\bmatrix{x_1'\cr x_2'}=
\bmatrix{ 
0 & 1 \cr
\frac{2}{1+t} & \frac{1-t}{1+t}
}
\bmatrix{x_1\cr x_2} 
+\bmatrix{ 0\cr \frac{6te^{2t}}{1+t} }.
$$
The general solutions of this system are
$\bmatrix{x_1(t)\cr x_2(t)} =
\bmatrix{ e^{2t}+ C_1(1+t^2)+C_2 e^{-t} \cr 
2e^{2t}+ 2C_1 t -C_2 e^{-t}}$.
Or, equivalently,
$\bmatrix{x_1(t)\cr x_2(t)} =\bmatrix{ e^{2t} \cr 2e^{2t}}+
C_1 \bmatrix{1+t^2 \cr 2t} +C_2\bmatrix{ e^{-t}\cr -e^{-t}}$.
	\end{enumerate}


\item
	\begin{enumerate}
	\item  
The general solutions: 
$\displaystyle y(t)=C_1 e^{-4t} +C_2 e^{-t/2}$,
where $C_1,C_2$ are free parameters.\\[1ex]
The solution satisfying $y(0)=-1,y'(0)=2$ is
$y(t)=-{3\over 7} e^{-4t} -{4\over 7} e^{-t/2}$.\\[1ex]
The equilibrium $(y,y')=(0,0)$ is an attractive improper node
and is asymptotically stable.
\medskip

\begin{minipage}{0.65\textwidth}
{\color{red}\small\em Notes:}
	{\small \color{blue}
The phase portrait
should show the following elements:
\begin{description}
\item{$\bullet$}
correct eigenspaces in the directions of 
$\bmatrix{1\cr -4}$ and $\bmatrix{1\cr -1/2}$;
\item{$\bullet$}
curved trajectories for solutions that are not on the eigenspaces;
\item{$\bullet$} 
at the equilibrium, all the curved trajectories are tangent 
to the eigenspace of $\lambda_2=-1/2$;
\item{$\bullet$}
and needless to say, the correct arrows
on all trajectories.
\end{description}}
\end{minipage}
\hfill
\begin{minipage}{0.3\textwidth}
 \includegraphics*[width=\textwidth]{testpr-2nd-ord-eq-attr-node.eps}
\end{minipage}
\medskip
  
	\item  
The general solutions: 
$\displaystyle y(t)=C_1 e^{2t} +C_2 e^{-4t}$, 
where $C_1,C_2$ are free parameters.\\[1ex]
The solution satisfying $y(0)=-1,y'(0)=2$ is 
$y(t)=-{1\over 3} e^{2t} -{2\over 3} e^{-4t}$.\\[1ex]
The equilibrium $(y,y')=(0,0)$ is a saddle
and is unstable.
\medskip

\begin{minipage}{0.65\textwidth}
{\color{red}\small\em Notes:}
	{\small \color{blue}
The phase portrait
should show the following elements:
\begin{description}
\item{$\bullet$}
the correct eigenspaces in the directions of 
$\bmatrix{1\cr 2}$ and $\bmatrix{1\cr -4}$;
\item{$\bullet$}
trajectories that are not on the eigenspaces are curved and transit from
the eigenspace of $\lambda_2=-4$ to the eigenspace of $\lambda_1=2$;
\item{$\bullet$}
and needless to say, the correct arrows
on all trajectories.
\end{description}}
\end{minipage}
\hfill
\begin{minipage}{0.3\textwidth}
\includegraphics*[width=\textwidth]{testpr-2nd-ord-eq-saddle.eps}
\end{minipage}
\medskip
  
\newpage

	\item  
The general solutions: 
$\displaystyle y(t)=C_1 e^{t/2} +C_2 e^{5t/2}$,
where $C_1,C_2$ are free parameters.\\
The solution satisfying $y(0)=-1,y'(0)=2$ is
$y(t)= -{9\over 4} e^{t/2} +{5\over 4} e^{5t/2}$.\\
The equilibrium $(y,y')=(0,0)$ is a repulsive improper node
and is unstable.
\medskip

\begin{minipage}{0.65\textwidth}
{\color{red}\small\em Notes:}
	{\small \color{blue}
The phase portrait
should show the following elements:
\begin{description}
\item{$\bullet$}
The correct eigenspaces in the directions of 
$\bmatrix{1\cr 1/2}$ and $\bmatrix{1\cr 5/2}$.
\item{$\bullet$}
Trajectories that are not on the eigenspaces are curved.
How do they curve?
E.g., in this problem, the curved trajectories should be tangent to the 
eigenspace of $\lambda_1=1/2$ near the origin.
\item{$\bullet$}
Needless to say, the figure should give
the correct correct arrows
on all trajectories.
\end{description}}
\end{minipage}
\hfill
\begin{minipage}{0.3\textwidth}
\centerline{\includegraphics*[width=\textwidth]{testpr-2nd-ord-eq-repul-node.eps} }
\end{minipage}
\medskip

	\item  
The general solutions: 
$\displaystyle y(t)=C_1   +C_2 e^{3t/2}$,
where $C_1,C_2$ are free parameters.\\
The solution satisfying $y(0)=-1,y'(0)=2$ is
$y(t)=-{7\over 3}   +{4\over 3} e^{3t/2}$.\\
The system has a repulsive line of equilibria.
Each equilibium $(y,y')=(c,0)$ is unstable.
\medskip

\begin{minipage}{0.65\textwidth}
{\color{red}\small\em Notes:}
	{\small \color{blue}
The phase portrait
should show the following elements:
\begin{description}
\item{$\bullet$}
the correct eigenspaces in the directions of 
$\bmatrix{1\cr 0}$ and $\bmatrix{1\cr 3/2}$;
\item{$\bullet$}
each nonequilibrium trajectory is a straight half-line
parallel to the eigenspace of $\lambda_2=3/2$
and emanates from an equilibrium on the eigenspace of $\lambda_1=0$;
\item{$\bullet$}
and needless to say, the correct arrows
on all trajectories.
\end{description}}
\end{minipage}
\hfill
\begin{minipage}{0.3\textwidth}
\centerline{\includegraphics*[width=\textwidth]{testpr-2nd-ord-eq-repul-line.eps} }
\end{minipage}
\medskip

	\item  
The general solutions: 
$\displaystyle y(t)=C_1 e^t\cos(2t)   +C_2 e^t\sin(2t)$,
where $C_1,C_2$ are free parameters.\\
The solution satisfying $y(0)=-1,y'(0)=2$ is
$y(t)= -e^t\cos(2t)   +{3\over 2} e^t\sin(2t)$.\\
The equilibrium $(y,y')=(0,0)$ is a repulsive focus
and is unstable.
\medskip

\begin{minipage}{0.6\textwidth}
{\color{red}\small\em Notes:}
	{\small \color{blue}
It's unrealistic to expect a hand-drawn figure 
to be as nice as computer graphics.
However, the phase portrait should show 
whether the trajectories are closed curves, 
spirals converging to the origin, 
or spirals leaving the origin \& go to infinity. 
Moreover, it should show correctly 
whether the spinning is clockwise or counterclockwise.}
\end{minipage}
\hfil
\begin{minipage}{0.3\textwidth}
\centerline{\includegraphics*[width=\textwidth]{testpr-2nd-ord-eq-repul-focus.eps} }
\end{minipage}
\medskip
 
	\item  
The general solutions: 
$\displaystyle y(t)=C_1  \cos(3t/2)   +C_2 \sin(3t/2)$.\\
The solution satisfying $y(0)=-1,y'(0)=2$ is
$y(t)= -\cos(3t/2) +\frac{4}{3}\sin(3t/2)$.\\
The origin $(y,y')=(0,0)$ is a center
and is stable but not asymptotically stable.
\medskip

\begin{minipage}{0.55\textwidth}
{\color{red}\small\em Notes:}
	{\small \color{blue}
It's unrealistic to expect a hand-drawn figure 
to be as nice as computer graphics.
However, the phase portrait should show the symmetric axes in 
the $x_1$ and $x_2$ directions. 
Moreover, the aspect ratio of the ellipses is given by:
$$\frac{(\mbox{the radius in the $x_1$ direction})}
{(\mbox{the radius in the $x_2$ direction})}
=\frac{1}{3/2}=\frac{2}{3}.$$
	}
\end{minipage}
\hfill
\begin{minipage}{0.3\textwidth}
\centerline{\includegraphics*[width=\textwidth]{testpr-2nd-ord-eq-center.eps} }
\end{minipage}
\medskip
  
	\item  
The general solutions: 
$\displaystyle y(t)=C_1 e^{-t/3}   +C_2 te^{-t/3}$,
where $C_1,C_2$ are free parameters.\\
The solution satisfying $y(0)=-1,y'(0)=2$ is
$y(t)= - e^{-t/3}   +\frac{5}{3} te^{-t/3}$.\\
The origin $(y,y')=(0,0)$ is an attractive degenerate node
and is asymptotically stable.
\medskip

\begin{minipage}{0.65\textwidth}
{\color{red}\small\em Notes:}
	{\small \color{blue}
The phase portrait
should show the following elements:
\begin{description}
\item{$\bullet$}
the correct eigenspace in the direction of 
$\bmatrix{1\cr -1/3}$;
\item{$\bullet$}
trajectories that are not on the eigenspace
are U-turn shaped curves,
converging to the origin;
\item{$\bullet$} 
at the equilibrium, all the curved trajectories are tangent 
to the eigenspace;
\item{$\bullet$}
and needless to say, the correct arrows
on all trajectories.
\end{description}}
\end{minipage}
\hfill
\begin{minipage}{0.3\textwidth}
\centerline{\includegraphics*[width=\textwidth]{testpr-2nd-ord-eq-attr-degen-node.eps} }
\end{minipage}

	\end{enumerate}


\item
	\begin{enumerate}
	\item
$\displaystyle
{\bf x}(t) = \left[ \matrix{
\displaystyle ({1\over 2}t+{1\over 8}) e^{3t} -{1\over 8}e^{-t}\cr
\cr
\displaystyle ({1\over 4}t-{1\over 16}) e^{3t} +{1\over 16}e^{-t}  }
\right]
$
	\item
$\displaystyle y(t)=3-4t+2t^2  -{3\over 10} \cos 4t +{ 2\over 5}\sin 4t
+{1\over 2} t^2 e^{-2t}
                        -{37 \over 10} e^{-2t} -3 t e^{-2t}$
	\item
$\displaystyle y(t)= -4 +8e^{-t/2}\ln\left( 2+e^{t/2} \right) 
+te^{t/2} -2e^{t/2}\ln\left( 2+e^{t/2} \right) 
+C_1 e^{t/2} +C_2 e^{-t/2} $
	\end{enumerate}




\item
${\bf x}(t)=\bmatrix{
e^{2t}\ln(1+e^t) \cr
te^{-2t}-e^{-2t}\ln(1+e^t) +e^{2t}\ln(1+e^t)  \cr
te^{-2t}-e^{-2t}\ln(1+e^t) +e^{2t}\ln(1+e^t) }
+C_1e^{-t}\bmatrix{1\cr 0\cr 1}
+C_2e^{-2t}\bmatrix{0\cr 1\cr 1}
+C_3e^{2t}\bmatrix{1\cr 1\cr 1}$

\item
$y(t)=
\frac{5}{16}\ln|\sin(2t)|
+\frac{5}{16}\cos(2t)\ln|\csc(2t)+\cot(2t)|
-\frac{5}{16}
+C_1+C_2\cos(2t)+C_3\sin(2t)$
% or, equivalently, 
% $y(t)=
% \frac{5}{16}\ln|\sin(2t)|
% -\frac{5}{16}\cos(2t)\ln|\tan t|
% -\frac{5}{16}
% +C_1+C_2\cos(2t)+C_3\sin(2t)$
%%%%%%%%%%%%
%%% another version: $y(t)=\frac{2}{27}\ln|\sin(3t)|  +\frac{2}{27}\cos(3t)\ln|\csc(3t)+\cot(3t)|  -\frac{2}{27}  +C_1+C_2\cos(3t)+C_3\sin(3t)$

\newpage 

\item
	\begin{enumerate}
	\item
${\bf x}'
=\bmatrix{ 0&0&1&0 \cr 0&0&0&1\cr 0&-1&0&0\cr -1&0&0&0}{\bf x}
+\bmatrix{ 0\cr 0\cr \cos t \cr \cos t}$
	\item
$M(t)=\bmatrix{
e^t  &  e^{-t} &  \cos t &  \sin t \cr
-e^t & -e^{-t} &  \cos t &  \sin t \cr
 e^t & -e^{-t} & -\sin t &  \cos t \cr
-e^t &  e^{-t} & -\sin t &  \cos t }$
	\item
${\bf u}'(t)=\bmatrix{0\cr 0\cr -\sin t \cos t \cr \cos^2 t}$
	\item
${\bf u}_p(t)=
\bmatrix{0\cr 0\cr
\frac{1}{4}\cos(2t) \cr \frac{1}{2}t +\frac{1}{4}\sin(2t) }$,
\quad
${\bf x}_p(t)=
\bmatrix{
\frac{1}{4}\cos t +\frac{1}{2} t\sin t \cr
\frac{1}{4}\cos t +\frac{1}{2} t\sin t \cr
\frac{1}{4}\sin t +\frac{1}{2} t\cos t \cr
\frac{1}{4}\sin t +\frac{1}{2} t\cos t }$
	\item
${\bf x}(t)=
\bmatrix{
\frac{1}{4}\cos t +\frac{1}{2} t\sin t \cr
\frac{1}{4}\cos t +\frac{1}{2} t\sin t \cr
\frac{1}{4}\sin t +\frac{1}{2} t\cos t \cr
\frac{1}{4}\sin t +\frac{1}{2} t\cos t }
+C_1 e^t   \bmatrix{1\cr -1\cr  1\cr -1}
+C_2 e^{-t}\bmatrix{1\cr -1\cr -1\cr  1}
+C_3 \bmatrix{ \cos t \cr \cos t \cr -\sin t \cr -\sin t}
+C_4 \bmatrix{ \sin t \cr \sin t \cr \cos t \cr \cos t}$
	\item
$y(t)=\frac{1}{4}\cos t +\frac{1}{2} t\sin t
+C_1 e^t +C_2 e^{-t}+C_3 \cos t +C_4 \sin t$,\\
$z(t)=\frac{1}{4}\cos t +\frac{1}{2} t\sin t
-C_1 e^t -C_2 e^{-t}+C_3 \cos t +C_4 \sin t$
	\end{enumerate}







\item
	\begin{enumerate}
	\item
The initial value problem is: 
$\displaystyle \frac{60}{32} y'' +120 y=0,\ 
y(0)=-1,\ y'(0)=2.$

The solution is $y(t)= -\cos(8 t) +{1 \over 4} \sin(8t)$~ft.

The amplitude $A={1\over 4}\sqrt{17}$~ft, the frequency $\omega=8$~rad/s,
and the period $T={\pi\over 4}$~s.
	\item
$\displaystyle {30g\over \pi^2}\approx 97.27$~lb
	\end{enumerate}
 

\item
	\begin{enumerate} 
	\item
The displacement from the equilibrium position is
$0.1e^{-t}\cos t+0.1e^{-t}\sin t$ (meters).
	\item
The displacement from the equilibrium position is
$0.2e^{-t} -0.1e^{-2t}$ (meters).
 	\end{enumerate}

\item
$y(t)=6t\sin(2t)$~in,
or, equivalently,
$y(t)={1\over 2}t\sin(2t)$~ft


\item
(a) $50y''+50y'+100y=10\cos(\omega t)$ \qquad
(b) $\frac{1}{10}\cos t +\frac{1}{10}\sin t$~meters

(c) Increases.\qquad
(d) $ -\frac{1}{20}\cos (2t) +\frac{1}{20}\sin (2t)$~meters \qquad
(e) Decreases.




\item
$\displaystyle \frac{ e^{-3s+12} - e^{-7s+28}  }{ s-4 }$
 
(Hint: You may use the definition of the Laplace transform \& carry out the integration directly. 
Or you may use the method of Section 5.5.)

\newpage

\item
$\displaystyle F(s)=\frac{360}{s^6}-\frac{14}{s^3}+\frac{9}{s}
+\frac{2}{s+3}+\frac{6}{(s-2)^4}
+\frac{4s}{s^2+36} -\frac{30}{s^2+36}$


\item
$\displaystyle \frac{s+1}{(s+1)^2 +9} +\frac{6s}{(s^2+9)^2} -\frac{42(s+2)}{[(s+2)^2 +9]^2}$


\item
$\displaystyle -5 +\frac{1}{40}t^5 +\frac{1}{2}e^{5t} t^2 +2e^{2t} -7e^{4t} +e^{-t}
+2\cos(\pi t) +\frac{1}{\pi}\sin(\pi t) 
-4e^{-3t}\cos(5t) +\frac{12}{5}e^{-3t}\sin(5t)$


\item
(a) $ sY(s)-7+2Y(s)=\frac{6}{s-3}$\qquad
(b) $ Y(s)=\frac{7}{s+2}+\frac{6}{(s+2)(s-3)}$\qquad
(c) $ y(t)=\frac{29}{5}e^{-2t} +\frac{6}{5}e^{3t}$

\item
(a) $ [s^2Y(s)+3s-2] +2[sY(s)+3] +Y(s)=\frac{8}{s-3}$\\
(b) $ Y(s)=-\frac{3s+4}{(s+1)^2}+\frac{8}{(s+1)^2(s-3)}$\\
(c) $ y(t)=-3te^{-t} -\frac{7}{2}e^{-t} +\frac{1}{2}e^{3t}$

\item
(a) $s^2 X(s)-s+2=-6X(s)+4Y(s),\quad sY(s)-4=5X(s)$\\
(b) $X(s)=\frac{s^2-2s+16}{s^3+6s-20}, Y(s)=\frac{4s^2+5s+14}{s^3+6s-20}$\\
(c) $x(t)=\frac{8}{9}e^{2t}+\frac{1}{9}e^{-t}\cos(3t)-\frac{11}{9}e^{-t}\sin(3t),
     y(t)=\frac{20}{9}e^{2t}+\frac{16}{9}e^{-t}\cos(3t)+\frac{7}{9}e^{-t}\sin(3t)$



