\newpage 
\ifnum \Version=1
\question[6] Consider the differential equation

$$y'' + 2y' + y = 6e^{-t}, \quad y=y(t)$$    

Solutions to the homogeneous problem are $y_1 = e^{-t}$ and $y_2 = te^{-t}$. 

\begin{parts}
    \part Determine a particular solution to the differential equation using variation of parameters. Do not use undetermined coefficients. \ifnum \Solutions=0 
    \vspace{16cm}
    \fi
    \part State the general solution to the differential equation.
\end{parts}
\ifnum \Solutions=1 {\color{DarkBlue} Solution written below. 
    \begin{figure}[h]
    \centering
    \includegraphics[width=16cm]{Images/ImgTest2VoP.jpg}
    \end{figure}  
} 
\else 
\vspace{3cm}
\fi
\fi


\ifnum \Version=2
\question[6] Consider the differential equation

    $$y'' + p(t)y' + q(t)y = 60t^3, \quad y=y(t)$$    
    
    Solutions to the corresponding homogeneous problem are $y_1 = 1$ and $y_2 = t^2$. 

    \begin{parts}
        \part Determine a particular solution to the differential equation using variation of parameters. Do not use the method of undetermined coefficients. 
        \ifnum \Solutions=0 
        \vspace{16cm}
        \fi
        \part State the general solution to the differential equation.
    \end{parts}
    \ifnum \Solutions=1 {\color{DarkBlue} 
    \input{2023Summer/Test2/SolPage2t3}
    } 
    \else 
    \fi    
\fi

\ifnum \Version=3
\question[6] Consider the differential equation

    $$y'' + p(t)y' + q(t)y = 60e^{-4t}, \quad y=y(t)$$    
    
    Solutions to the corresponding homogeneous problem are $y_1 = e^t$ and $y_2 = 1$. 
    
    \begin{parts}
        \part Determine a particular solution to the differential equation using variation of parameters. Do not use the method of undetermined coefficients. 
        \ifnum \Solutions=0 
        \vspace{16cm}
        \fi
        \part State the general solution to the differential equation.
    \end{parts}
    \ifnum \Solutions=1 {\color{DarkBlue}  
    \input{2023Summer/Test2/SolPage24t}
    } 
    \else 
    \fi        
\fi


\ifnum \Version=4
\question[6] Consider the differential equation

    $$y'' + p(t)y' + q(t)y = 60t^3, \quad y=y(t)$$    
    
    Solutions to the corresponding homogeneous problem are $y_1 = 1$ and $y_2 = t^2$. 
    
    \begin{parts}
        \part Determine a particular solution to the differential equation using variation of parameters. Do not use the method of undetermined coefficients. 
        \ifnum \Solutions=0 
        \vspace{16cm}
        \fi
        \part State the general solution to the differential equation.
    \end{parts}
    \ifnum \Solutions=1 {\color{DarkBlue}  
    \input{2023Summer/Test2/SolPage2t3}
    } 
    \else 
    \fi
\fi

\ifnum \Version=5
\question[6] Consider the differential equation

    $$y'' + p(t)y' + q(t)y = 60e^{-4t}, \quad y=y(t)$$    
    
    Solutions to the corresponding homogeneous problem are $y_1 = e^t$ and $y_2 = 1$. 

    \begin{parts}
        \part Determine a particular solution to the differential equation using variation of parameters. Do not use the method of undetermined coefficients. 
        \ifnum \Solutions=0 
        \vspace{16cm}
        \fi
        \part State the general solution to the differential equation.
    \end{parts}
    \ifnum \Solutions=1 {\color{DarkBlue}  
    \input{2023Summer/Test2/SolPage24t}
    } 
    \else 
    \fi    
\fi



\ifnum \Version>5
\question[4] Consider the first order system \[\vec{x} \, ' = \left( \begin{array}{rr} 2 & 4 \\ 4 & 2 \end{array} \right) \vec{x}  + \begin{pmatrix} 24\\0\end{pmatrix}  \]
    
    Solutions to the corresponding homogeneous problem are $\vec x_1 = e^{-2t}\begin{pmatrix} 1\\-1\end{pmatrix}$ and $\vec x_2 = e^{6t}\begin{pmatrix} 1\\1\end{pmatrix}$. 

    \begin{parts}
        \part Determine a particular solution to the differential equation using variation of parameters. Do not use the method of undetermined coefficients. 
\ifnum \Solutions=0 \vspace{17cm}\fi
        \part State the general solution to the system of differential equations. 
    \end{parts}
    \ifnum \Solutions=1 {\color{DarkBlue}   
    
    \begin{itemize}
        \item \textbf{Fundamental Matrix}\\
        The fundamental matrix \(X(t)\) is constructed by placing the solutions \(\vec{x}_1\) and \(\vec{x}_2\) as columns in a matrix. Thus,
        
        \[
        X(t) = \begin{pmatrix} \vec{x}_1 & \vec{x}_2 \end{pmatrix} = \begin{pmatrix} e^{-2t} & e^{6t} \\ -e^{-2t} & e^{6t} \end{pmatrix}
        \]
        \item \textbf{Inverse}\\
        \begin{align*}
            \det(X(t)) &= e^{-2t} \cdot e^{6t} - e^{6t} \cdot (-e^{-2t}) = e^{4t} + e^{4t} = 2e^{4t}\\
            X^{-1} &= \frac{1}{2e^{4t}} \begin{pmatrix} e^{6t} & -e^{6t} \\ e^{-2t} & e^{-2t} \end{pmatrix}
        = \frac{1}{2} \begin{pmatrix} e^{2t} & -e^{2t} \\ e^{-6t} & e^{-6t} \end{pmatrix}
        \end{align*}
        
        \item \textbf{Particular}\\
        \begin{align}
            \vec x_p &= X \int X^{-1} g \, dt \\
            &= X \int \frac{1}{2} \begin{pmatrix} e^{2t} & -e^{2t} \\ e^{-6t} & e^{-6t} \end{pmatrix} \begin{pmatrix} 24 \\ 0 \end{pmatrix} \, dt \\
            & = X \int \begin{pmatrix} 12e^{2t} \\ 12e^{-6t} \end{pmatrix} \, dt \\
            &= \begin{pmatrix} e^{-2t} & e^{6t} \\ -e^{-2t} & e^{6t} \end{pmatrix} \begin{pmatrix} 6e^{2t} + C_1 \\ -2e^{-6t} + C_2 \end{pmatrix} \\
            &=  \begin{pmatrix} 4 + C_1 e^{-2t} + C_2 e^{6t} \\ -8 - C_1 e^{-2t} + C_2 e^{6t} \end{pmatrix}
        \end{align}  
        It is not necessary to keep the $C_1$ and $C_2$ terms, they can be ignored. 
        \item \textbf{General Solution}
        \begin{align}
            \vec x = \vec x_h + \vec x_p = c_1 e^{-2t}\begin{pmatrix} 1\\-1\end{pmatrix} + c_2 e^{6t}\begin{pmatrix} 1\\1\end{pmatrix} + \begin{pmatrix} 4\\-8\end{pmatrix}
        \end{align}

    \end{itemize}




    } 
    \else 
    \fi    
\fi

