\ifnum \Version=1
\question[2] You do not need to show your work for this question. Complete the table below by calculating the inverse Laplace Transform of the following functions. Do not use the convolution theorem. 
\vspace{-0.4cm}
\setlength{\extrarowheight}{0.60cm}
\begin{center}
\hspace{-.9cm}\begin{tabular}{ p{0.20cm} p{4cm} p{7cm}  }
    & $F(s) = \mathcal{L} [f(t)]$& $f(t)$   \\[2pt] \hline 
    a) & $\displaystyle F(s) = \frac{(s-2)e^{-s}}{(s-2)^2+9}$ & $f(t) = $ \ifnum \Solutions=1 {\color{DarkBlue}  $u_1e^{2(t-1)}\cos(3(t-1))$ }\fi \\[4pt] 
    b) & $\displaystyle F(s) = \frac{s+4}{s^2+4}$ & $f(t) = $ \ifnum \Solutions=1 {\color{DarkBlue} $\cos(2t) + 2\sin(2t)$}\fi \\[8pt]      
    \hline
\end{tabular}
\end{center}
\setlength{\extrarowheight}{0.0cm}
\ifnum \Solutions=1 {\color{DarkBlue} 
Note that $\displaystyle \frac{s+4}{s^2+4} = \frac{s}{s^2+4} + 2\frac{2}{s^2+4}$.
} 
\else 
\fi
\fi 



\ifnum \Version=2
\question[2] You do not need to show your work for this question. Complete the table below by calculating the inverse Laplace Transform of the following functions. Do not use the convolution theorem. 
\vspace{-0.4cm}
\setlength{\extrarowheight}{0.60cm}
\begin{center}
\hspace{-.9cm}\begin{tabular}{ p{0.20cm} p{4cm} p{7cm}  }
    & $F(s) = \mathcal{L} [f(t)]$& $f(t)$   \\[2pt] \hline 
    a) & $\displaystyle F(s) = \frac{4e^{-2s}}{s^2+9}$ & $f(t) = $ \ifnum \Solutions=1 {\color{DarkBlue}  $\frac43 u_2 \sin(3(t-2))$ }\fi \\[4pt] 
    b) & $\displaystyle F(s) = \frac{s+1}{s^2-1}$ & $f(t) = $ \ifnum \Solutions=1 {\color{DarkBlue} $e^t$}\fi \\[8pt]      
    \hline
\end{tabular}
\end{center}
\setlength{\extrarowheight}{0.0cm}
\ifnum \Solutions=1 {\color{DarkBlue} 
Note that $\displaystyle \frac{s+1}{s^2-1} = \frac{s+1}{(s+1)(s-1)} =\frac{1}{s-1}$.
} 
\else 
\fi
\fi 



\ifnum \Version=3
\question[2] You do not need to show your work for this question. Complete the table below by calculating the inverse Laplace Transform of the following functions. Do not use the convolution theorem. 
\vspace{-0.4cm}
\setlength{\extrarowheight}{0.60cm}
\begin{center}
\hspace{-.9cm}\begin{tabular}{ p{0.20cm} p{4cm} p{7cm}  }
    & $F(s) = \mathcal{L} [f(t)]$& $f(t)$   \\[2pt] \hline 
    a) & $\displaystyle F(s) = \frac{4e^{-2s}}{s^2+9}$ & $f(t) = $ \ifnum \Solutions=1 {\color{DarkBlue}  $\frac43 u_2 \sin(3(t-2))$ }\fi \\[4pt] 
    b) & $\displaystyle F(s) = \frac{8}{(s+1)^2+4}$ & $f(t) = $ \ifnum \Solutions=1 {\color{DarkBlue} $4e^{-t}\sin(2t)$}\fi \\[8pt]      
    \hline
\end{tabular}
\end{center}
\setlength{\extrarowheight}{0.0cm}
\fi 



\ifnum \Version=4
\question[2] You do not need to show your work for this question. Complete the table below by calculating the inverse Laplace Transform of the following functions. Do not use the convolution theorem. 
\vspace{-0.4cm}
\setlength{\extrarowheight}{0.60cm}
\begin{center}
\hspace{-.9cm}\begin{tabular}{ p{0.20cm} p{4cm} p{7cm}  }
    & $F(s) = \mathcal{L} [f(t)]$& $f(t)$   \\[2pt] \hline 
    a) & $\displaystyle F(s) = \frac{6se^{-8s}}{s^2+4}$ & $f(t) = $ \ifnum \Solutions=1 {\color{DarkBlue}  $61u_8 \cos(2(t-8))$ }\fi \\[4pt] 
    b) & $\displaystyle F(s) = \frac{s+2}{(s+1)^2+1}$ & $f(t) = $ \ifnum \Solutions=1 {\color{DarkBlue} $e^{-t}(\cos t + \sin t)$}\fi \\[8pt]      
    \hline
\end{tabular}
\setlength{\extrarowheight}{0.0cm}
\end{center}
\ifnum \Solutions=1 {\color{DarkBlue} 
Note that $\frac{s+2}{(s+1)^2+1} = \frac{s+1}{(s+1)^2+1} + \frac{1}{(s+1)^2+1}$. 
} 
\else 
\fi
\fi 




\ifnum \Version=6
\question[2] You do not need to show your work for this question. Complete the table below by calculating the inverse Laplace Transform of the following functions. Do not use the convolution theorem. 
\vspace{-0.4cm}
\setlength{\extrarowheight}{0.60cm}
\begin{center}
\hspace{-.9cm}\begin{tabular}{ p{0.20cm} p{4cm} p{7cm}  }
    & $F(s) = \mathcal{L} [f(t)]$& $f(t)$   \\[2pt] \hline 
    a) & $\displaystyle F(s) = \frac{4e^{-\pi s}}{(s+1)^2+1}$ & $f(t) = $ \ifnum \Solutions=1 {\color{DarkBlue}  $4e^{-(t-\pi)}\sin(t-\pi)u_{\pi}$ }\fi \\[4pt] 
    b) & $\displaystyle F(s) = \frac{8}{4s^2+4s+17}$ & $f(t) = $ \ifnum \Solutions=1 {\color{DarkBlue} $e^{-t/2}\sin2t$}\fi \\[8pt]      
    \hline
\end{tabular}
\end{center}
\setlength{\extrarowheight}{0.0cm}
\ifnum \Solutions=1 {\color{DarkBlue} 
Note that:
\begin{align}
    \frac{8}{4s^2+4s+17} &= \frac44 \, \cdot \, \frac{2}{s^2+s+17/4} = \frac{2}{(s+1/2)^2 +2^2} = \mathcal{L}[e^{-t/2}\sin2t]
\end{align}
} 
\else 
\fi
\fi 


% \ifnum \Version=6
% \question[2] You do not need to show your work for this question. Complete the table below by calculating the inverse Laplace Transform of the following functions. Do not use the convolution theorem. 
% \vspace{-0.4cm}
% \setlength{\extrarowheight}{0.60cm}
% \begin{center}
% \hspace{-.9cm}\begin{tabular}{ p{0.20cm} p{4cm} p{7cm}  }
%     & $F(s) = \mathcal{L} [f(t)]$& $f(t)$   \\[2pt] \hline 
%     a) & $\displaystyle F(s) = \frac{4e^{-\pi s}}{(s+1)^2+1}$ & $f(t) = $ \ifnum \Solutions=1 {\color{DarkBlue}  $e^{-(t-\pi)}\sin(t-\pi)u_{\pi}$ }\fi \\[4pt] 
%     b) & $\displaystyle F(s) = \frac{8}{4s^2+4s+17}$ & $f(t) = $ \ifnum \Solutions=1 {\color{DarkBlue} $2e^{-t/2}\sin2t$}\fi \\[8pt]      
%     \hline
% \end{tabular}
% \end{center}
% \setlength{\extrarowheight}{0.0cm}
% \ifnum \Solutions=1 {\color{DarkBlue} 
% Note that:
% \begin{align}
%     \frac{8}{4s^2+4s+17} &= \frac{4}{s^2+s+17/4} = 2\frac{2}{(s+1/2)^2 +2^2} = \mathcal{L}[2e^{-t/2}\sin2t]
% \end{align}
% } 
% \else 
% \fi
% \fi 


\ifnum \Version=7
\question[2] You do not need to show your work for this question. Complete the table below by calculating the inverse Laplace Transform of the following functions. Do not use the convolution theorem. 
\vspace{-0.4cm}
\setlength{\extrarowheight}{0.60cm}
\begin{center}
\hspace{-.9cm}\begin{tabular}{ p{0.20cm} p{4cm} p{7cm}  }
    & $F(s) = \mathcal{L} [f(t)]$& $f(t)$   \\[2pt] \hline 
    a) & $\displaystyle F(s) = \frac{12e^{-\pi s}}{(s+1)^2+1}$ & $f(t) = $ \ifnum \Solutions=1 {\color{DarkBlue}  $12e^{-(t-\pi)}\sin(t-\pi)u_{\pi}$ }\fi \\[4pt] 
    b) & $\displaystyle F(s) = \frac{16}{4s^2+4s+17}$ & $f(t) = $ \ifnum \Solutions=1 {\color{DarkBlue} $2e^{-t/2}\sin2t$}\fi \\[8pt]      
    \hline
\end{tabular}
\end{center}
\setlength{\extrarowheight}{0.0cm}
\ifnum \Solutions=1 {\color{DarkBlue} 
Note that:
\begin{align}
    \frac{16}{4s^2+4s+17} &= \frac{4}{4} \, \cdot \, \frac{4}{s^2+s+17/4} = 2 \, \cdot \, \frac{2}{(s+1/2)^2 +2^2} = \mathcal{L}[2e^{-t/2}\sin2t]
\end{align}
} 
\else 
\fi
\fi 
